Accept submission 2825eaf2-7b45-48f5-84d0-1c2dc8b171a9
Co-authored-by: Meganpark980320 <186258306+Meganpark980320@users.noreply.github.com>

Challenge/Ripemd160/Submission/Proofs/Bytecode/JointRightPackRaw.lean
@@ -38,7 +38,7 @@ def template : List Instr :=
     .op .OR,
     .op .XOR,
     .op .ADD,
-    .push ⟨2, by decide⟩ (UInt256.ofNat 630),
+    .push ⟨1, by decide⟩ (UInt256.ofNat 252),
     .op .MLOAD,
     .op .ADD,
     .op .ADD,
@@ -88,7 +88,7 @@ def actualOutput (memory : ByteArray) (x : Input) (rho : List UInt256) : List UI
   [ (UInt256.ofNat 95780971281817308448866066055358605703522837925462015),
     (UInt256.ofNat 95780971281817308448866066055358605703522833630494720),
     (UInt256.lor x.h4 (UInt256.shiftLeft x.rd (UInt256.ofNat 144))),
-    (UInt256.lor x.h1 (UInt256.shiftLeft (UInt256.land x.lower (UInt256.add x.re (UInt256.shiftRight (UInt256.mul x.factor (UInt256.land x.lower (UInt256.add (UInt256.add (MachineState.readWord memory 630) (UInt256.add (UInt256.xor (UInt256.lor x.rc (UInt256.lnot x.rd)) x.rb) x.ra)) x.k))) (UInt256.ofNat 29)))) (UInt256.ofNat 144))),
+    (UInt256.lor x.h1 (UInt256.shiftLeft (UInt256.land x.lower (UInt256.add x.re (UInt256.shiftRight (UInt256.mul x.factor (UInt256.land x.lower (UInt256.add (UInt256.add (MachineState.readWord memory 252) (UInt256.add (UInt256.xor (UInt256.lor x.rc (UInt256.lnot x.rd)) x.rb) x.ra)) x.k))) (UInt256.ofNat 29)))) (UInt256.ofNat 144))),
     (UInt256.lor x.h0 (UInt256.shiftLeft x.re (UInt256.ofNat 144))),
     (UInt256.lor x.h3 (UInt256.shiftLeft (UInt256.shiftRight (UInt256.mul x.factor x.rc) (UInt256.ofNat 28)) (UInt256.ofNat 144))),
     (UInt256.lor x.h2 (UInt256.shiftLeft x.rb (UInt256.ofNat 144))),
@@ -111,7 +111,7 @@ def roundT (memory : ByteArray) (x : Input) : UInt256 :=
   UInt256.land x.lower (UInt256.add x.re
     (UInt256.shiftRight (UInt256.mul x.factor
       (UInt256.land x.lower (UInt256.add x.k
-        (UInt256.add (MachineState.readWord memory 630)
+        (UInt256.add (MachineState.readWord memory 252)
           (UInt256.add (UInt256.xor (UInt256.lor x.rc (UInt256.lnot x.rd)) x.rb) x.ra)))))
       (UInt256.ofNat 29)))
 def packed (a b : UInt256) : UInt256 :=
